{
 "cells": [
  {
   "cell_type": "markdown",
   "metadata": {},
   "source": [
    "**Q1.** Find the value of T(2) for the recurrence relation **T(n) = 3T(n-1) + 12*n**, given that **T(0)=5**\n",
    "\n",
    "**Solution:**\n",
    "\n",
    "Given: T(n) = 3T(n-1) + 12*n, T(0)=5\n",
    "To find: T(2) = ?\n",
    "\n",
    "put n = 1 in the given equation,\n",
    "\n",
    "* T(1) = 3T(1 - 1) + 12 * 1\n",
    "\n",
    "* => T(1) = 3T(0) + 12 = 3 * 5 + 12 \n",
    "     \n",
    "* => T(1) = 27    (given T(0) = 5)\n",
    "\n",
    "therefore, T(1) = 27\n",
    "\n",
    "Now, put n = 2 in the given equation,\n",
    "\n",
    "* T(2) = 3T(2-1) + 12 * 2 \n",
    "     \n",
    "* => T(2) = 3T(1) + 24\n",
    "     \n",
    "* => T(2) = 3*27 + 24               (using, T(1) = 27)\n",
    "     \n",
    "* => T(2) = 105\n",
    "\n",
    "Hence, **T(2) = 105**"
   ]
  },
  {
   "cell_type": "markdown",
   "metadata": {},
   "source": [
    "**Q2.** Given a recurrence relation, solve it using the substitution method:\n",
    "\n",
    "**a. T(n) = {1 ; n=1, T(n-1) + c ; n > 1}**\n",
    "\n",
    "**Solution:** According to ques,\n",
    "\n",
    "* T(n) = T(n-1) + c   ...(i)\n",
    "\n",
    "* T(n-1) = T(n-2) + c     ...(replacing n by (n-1) in (i) )\n",
    "\n",
    "* therefore, T(n) = T(n-2) + 2*c  ...(substituting the value of T(n-1) in (i))\n",
    "\n",
    "from this we can visualise that, the general equation of T(n) will be:\n",
    "* T(n) = T(n-k) + k*c   ...(ii)\n",
    "\n",
    "According to given initial condition T(n)=1 if n = 1, so we can assume that\n",
    "* if, n-k = 1 then, T(n-k) = 1 and k = n - 1        ...(iii)\n",
    "* Therefore, T(n) = 1 + (n-1)*c = O(n)    ...( substituting (iii) in (ii) )\n",
    "\n",
    "Hence, **Time complexity = O(n)**"
   ]
  },
  {
   "cell_type": "markdown",
   "metadata": {},
   "source": [
    "**b. T(n) = {1 ; n=1, 2*T(n/2) + n ; n > 1}**\n",
    "\n",
    "**Solution:** According to ques,\n",
    "* T(n) = 2*T(n/2) + n    ...(i)\n",
    "\n",
    "put n = n/2 in i, we get\n",
    "* T(n/2) = 2T(n/2^2) + n/2  ...(ii)\n",
    "\n",
    "from i and ii,\n",
    "* T(n) = 2^2T(n/2^2) + 2*n  ...(iii)\n",
    "\n",
    "so from (i), (ii) and, (iii) we can assume that the general equation of T(n) will be:\n",
    "* T(n) = 2^k*T(n/2^k) + k.n  ...(iv)\n",
    "\n",
    "According to given initial condition\n",
    "* T(n) = 1 if n = 1\n",
    "* therefore,\n",
    "* if n/2^k = 1 then, T(n/2^k) = 1 and k = log(n) of base 2      ...(v)\n",
    "\n",
    "from (v) and (iv),\n",
    "* T(n) = 2^(log(n) of base 2).T(1) + (log(n) of base 2)*n\n",
    "* by solving this we get,\n",
    "* T(n) = n + n.(log(n) of base 2)\n",
    "* The dominant term in this expression is n.(log(n) of base 2) because it grows more quikly that the linear term n as n becomes large.\n",
    "\n",
    "thus, **Time complexity = O(n*log(n) of base 2)** \n",
    "\n"
   ]
  },
  {
   "cell_type": "markdown",
   "metadata": {},
   "source": [
    "**c. T(n) = {1 ; n=1, 2T(n/2) + c ; n > 1}**\n",
    "\n",
    "**Solution:** According to ques,\n",
    "* T(n) = 2.T(n/2) + c    ...(i)\n",
    "\n",
    "substitute n = n/2 in (i), we get\n",
    "* T(n/2) = 2.T(n/2^2) + c    ...(ii)\n",
    "\n",
    "from (ii) and (i),\n",
    "* T(n) = 2^2.T(n / 2^2) + { 2^(2-1) + 2^(2-2) }.c ...(iii)\n",
    "\n",
    "from (i), (ii) and, (iii) we can assume that after k iterations\n",
    "* T(n) = 2^k.T(n / 2^k) + { 2^(k-1) + 2^(k-2) + 2^(k-3) + ... + 2^(k-k) }.c\n",
    "* => T(n) = 2^k.T(n/2^k) + [ {2^(k-1).(2^(-k) - 1)} / (2^(-1)-1) ]  ...{using formula, a^1 + a^2 + ... + a^n = a(r^n - 1)/(r-1), where r is common ratio}\n",
    "* => T(n) = 2^k.T(n/2^k) + 2^k - 1    ...(iv)\n",
    "\n",
    "from the given initial condition i.e., T(n) = 1 if n = 1, so we can assume that\n",
    "* T(n/2^k) = 1 if n/2^k = 1 ,therfore n = 2^k or k = log(n) of base 2   ...(v)\n",
    "\n",
    "from (iv) and (v)\n",
    "* T(n) = n.T(1) + n - 1 = 2.n - 1 ...(vi)\n",
    "\n",
    "from vi we can see that it is a linear time complexity, therefore\n",
    "\n",
    "**Time complexity = O(n)**"
   ]
  },
  {
   "cell_type": "markdown",
   "metadata": {},
   "source": [
    "**d. T(n) = {1 ; n=1, T(n/2) + c ; n>1}**\n",
    "\n",
    "**Solution:** According to ques,\n",
    "\n",
    "we have,\n",
    "* T(n) = T(n/2) + c ...(i)\n",
    "\n",
    "substitute *n = n/2* in (i), we get\n",
    "* T(n) = T(n/2^2) + 2.c ...(ii)\n",
    "\n",
    "from (i) and (ii), we can assume that after k iterations\n",
    "* T(n) = T(n/2^k) + k.c ...(iii)\n",
    "\n",
    "from the given initial condition, T(n) = 1 if n = 1. so, we can assume that in (iii)\n",
    "* if n/2^k = 1 then, T(n/2^k) = 1, n = 2^k and k = log(n) of base 2 ...(iv)\n",
    "\n",
    "thus, from (iii) and (iv)\n",
    "* T(n) = 1 + {log(n) of base 2}.c ...(v)\n",
    "\n",
    "Hence, according to equation v\n",
    "* **Time complexity = O(logn of base 2)**"
   ]
  },
  {
   "cell_type": "markdown",
   "metadata": {},
   "source": [
    "**Q3.** Given a recurrence relation, solve it using the recursive tree approach:"
   ]
  },
  {
   "cell_type": "markdown",
   "metadata": {},
   "source": [
    "**a. T(n) = {1; n = 1, 2T(n-1) + 1 ; n>1}**\n",
    "\n",
    "**solution:** According to ques,\n",
    "we have,\n",
    "* T(n) = 2T(n-1) + 1 ... (i)\n",
    "\n",
    "replace n by n-1 in (i), we get\n",
    "* T(n-1) = 2T(n-2) + 1  ...(ii)\n",
    "\n",
    "put the value of T(n-1) from (ii) in (i), we get\n",
    "* T(n) = 2^2T(n-2) + 2 + 1 ...(iii)\n",
    "\n",
    "from (i) and (iii) we can assume that after k iterations\n",
    "* T(n) = 2^kT(n-k) + 2^(k-1) + 2^(k-2) + ... + 2^(k-k)\n",
    "* => T(n) = 2^kT(n-k) + 2^(k-1)(1 - 2^-k)/2^-1  ...{using formula, a^1 + a^2 + ... + a^n = a(r^n - 1)/(r-1), where r is common ratio}\n",
    "* => T(n) = 2^kT(n-k) + 2^k - 1 ...(iv)\n",
    "\n",
    "from the given initial condition, T(n) = 1 if n = 1. therefore\n",
    "* if T(n-k) = 1 then, n-k = 1 and k = n-1   ...(v)\n",
    "\n",
    "from v and iv\n",
    "* T(n) = 2^(n-1)*1 + 2^(n-1) - 1\n",
    "* => T(n) = 2^n - 1 ...(vi)\n",
    "\n",
    "hence, from vi\n",
    "* **Time complexity = O(2^n)**"
   ]
  },
  {
   "cell_type": "markdown",
   "metadata": {},
   "source": [
    "**b. T(n) = {1; n = 1, 2T(n/2) + n ; n>1}**\n",
    "\n",
    "**solution:** According to ques,\n",
    "we have,\n",
    "* T(n) = 2T(n/2) + n    ...(i)\n",
    "\n",
    "replace n by n/2 in (i), we get\n",
    "* T(n/2) = 2T(n/2^2) + n/2  ...(ii)\n",
    "\n",
    "substitute the value of T(n/2) form (ii) in (i), we get\n",
    "* T(n) = 2^2T(n/2^2) + 2n   ...(iii)\n",
    "\n",
    "from (i) and (iii) we can assume that after k iterations\n",
    "* T(n) = 2^kT(n/2^k) + k*n  ...(iv)\n",
    "\n",
    "from the given initial condition T(n)=1, if n=1, therefore\n",
    "* if T(n/2^k) = 1 then, n/2^k = 1, 2^k = n and , k = logn of base 2   ...(v)\n",
    "\n",
    "from (v) and (iv), we get\n",
    "* T(n) = n.1 + n.(logn of base 2)\n",
    "* => T(n) = n + n.(logn of base 2)  ...(vi)\n",
    "* The dominant term in this expression is n.(log(n) of base 2) because it grows more quikly that the linear term n as n becomes large.\n",
    "\n",
    "Therefore, **Time complexity = O(n . (logn of base 2) )**"
   ]
  }
 ],
 "metadata": {
  "language_info": {
   "name": "python"
  }
 },
 "nbformat": 4,
 "nbformat_minor": 2
}
